coq-verification/src/Concrete/Assumptions/Addr.v
@@ -20,9 +20,13 @@ Axiom pa_difference : paddr_t -> paddr_t -> size_t.
 
 Axiom ipa_addr : ipaddr_t -> uintpaddr_t.
 
+Axiom va_init : uintvaddr_t -> vaddr_t.
+
 Axiom ipa_add : ipaddr_t -> size_t -> ipaddr_t.
 
 Axiom va_from_pa : paddr_t -> vaddr_t.
+
+Axiom pa_from_va : vaddr_t -> paddr_t.
 
 Axiom pa_from_ipa : ipaddr_t -> paddr_t.
 
